Some work on relation for beta equivalence

extraction/theories/OptimizeCorrectness.v
@@ -9,6 +9,7 @@ From Coq Require Import Bool.
 From Coq Require Import String.
 From Coq Require Import List.
 From Coq Require Import Psatz.
+From Coq Require Import RelationClasses.
 From Equations Require Import Equations.
 From MetaCoq.Erasure Require Import EAstUtils.
 From MetaCoq.Erasure Require Import ECSubst.
@@ -816,6 +817,80 @@ Context (ind_masks : list (kername * mib_masks)).
 Context (const_masks : list (kername * bitmask)).
 Notation dearg := (dearg ind_masks const_masks).
 Notation dearg_aux := (dearg_aux ind_masks const_masks).
+
+Reserved Infix "β=" (at level 70, right associativity).
+
+Inductive betaeq : term -> term -> Prop :=
+| betaeq_beta na body arg arg' sub :
+    arg β= arg' ->
+    sub β= subst1 arg' 0 body ->
+    tApp (tLambda na body) arg β= sub
+| betaeq_box : tBox β= tBox
+| betaeq_rel i : tRel i β= tRel i
+| betaeq_var id : tVar id β= tVar id
+| betaeq_evar i ts ts' :
+    Forall2 betaeq ts ts' ->
+    tEvar i ts β= tEvar i ts'
+| betaeq_lambda na body body' :
+    body β= body' ->
+    tLambda na body β= tLambda na body'
+| betaeq_let_in na val val' body body' :
+    val β= val' ->
+    body β= body' ->
+    tLetIn na val body β= tLetIn na val' body'
+| betaeq_app hd hd' arg arg' :
+    hd β= hd' ->
+    arg β= arg' ->
+    tApp hd arg β= tApp hd' arg'
+| betaeq_const kn : tConst kn β= tConst kn
+| betaeq_construct ind c : tConstruct ind c β= tConstruct ind c
+| betaeq_case ind npars disc disc' brs brs' :
+    disc β= disc' ->
+    betaeq_branches brs brs' ->
+    tCase (ind, npars) disc brs β= tCase (ind, npars) disc' brs'
+| betaeq_proj p t t' :
+    t β= t' ->
+    tProj p t β= tProj p t'
+| betaeq_fix defs defs' i :
+    betaeq_defs defs defs' ->
+    tFix defs i β= tFix defs' i
+| betaeq_cofix defs defs' i :
+    betaeq_defs defs defs' ->
+    tCoFix defs i β= tCoFix defs' i
+
+with betaeq_branches : list (nat × term) -> list (nat × term) -> Prop :=
+| betaeq_branches_nil : betaeq_branches [] []
+| betaeq_branches_cons ar t t' brs brs' :
+    t β= t' ->
+    betaeq_branches brs brs' ->
+    betaeq_branches ((ar, t) :: brs) ((ar, t') :: brs')
+
+with betaeq_defs : mfixpoint term -> mfixpoint term -> Prop :=
+| betaeq_defs_nil : betaeq_defs [] []
+| betaeq_defs_cons dname rarg dbody dbody' defs defs' :
+    dbody β= dbody' ->
+    betaeq_defs defs defs' ->
+    betaeq_defs
+      ({| dname := dname; dbody := dbody; rarg := rarg |} :: defs)
+      ({| dname := dname; dbody := dbody'; rarg := rarg |} :: defs')
+
+where "t β= t'" := (betaeq t t').
+
+Scheme betaeq_mind := Induction for betaeq Sort Prop
+  with betaeq_branches_mind := Induction for betaeq_branches Sort Prop
+  with betaeq_defs_mind := Induction for betaeq_defs Sort Prop.
+
+Fixpoint betaeq_refl (t : term) {struct term} : t β= t :=
+  match t with
+  | tBox =>
+with betaeq_branches_refl (brs : list (nat × term)) : betaeq_branches brs brs
+with betaeq_defs_refl (defs : mfixpoint term) : betaeq_defs defs defs.
+
+Global Instance betaeq_equivalence : Coq.Classes.RelationClasses.Equivalence betaeq.
+Proof.
+  constructor.
+  - intros x.
+    induction x.
 
 Lemma dearg_mkApps hd args :
   dearg (mkApps hd args) = dearg_aux (map dearg args) hd.
